spec_streebog_xlps.v
@@ -8,6 +8,8 @@ Require Import functional_spec.
 
 Import ListNotations.
 
+(* Check (@nil (list val)).  *)
+
 Definition tuint512 := Tstruct _streebog_uint512 noattr.
 
 Definition block512_to_chunks (b : block512) : list Z :=
@@ -16,23 +18,37 @@ Definition block512_to_chunks (b : block512) : list Z :=
 Definition block512_to_vals (b : block512) : list val :=
   map (fun x => Vlong (Int64.repr x)) (block512_to_chunks b).
 
+Definition Ax_to_vals (a : list (list int64)) : list (list val) :=
+  map (fun i => map (fun j => Vlong j) i) a.
+
+
+Definition gen_Ax : list (list int64) :=
+  map (fun i =>
+         map (fun j =>
+                tableLPS_i_j (Z.of_nat i) (Z.of_nat j))
+             (seq 0 256))
+      (seq 0 8).
+
 Definition streebog_xlps_spec :=
   DECLARE _streebog_xlps
   WITH sh_r : share, sh_w : share,
        x : val, y : val, z : val,
-       x_content : block512, y_content : block512, z_content : block512
+       x_content : block512, y_content : block512, z_content : block512,
+       Ax : val
   PRE [tptr tuint512, tptr tuint512, tptr tuint512]
     PROP(readable_share sh_r; writable_share sh_w)
     PARAMS (x; y; z)
     SEP (data_at sh_r tuint512 (block512_to_vals x_content) x;
          data_at sh_r tuint512 (block512_to_vals y_content) y;
-         data_at sh_w tuint512 (block512_to_vals z_content) z)
+         data_at sh_w tuint512 (block512_to_vals z_content) z;
+         data_at sh_r (tarray (tarray tulong 256) 8) (Ax_to_vals gen_Ax) Ax)
   POST [tvoid]
     PROP()
     RETURN()
     SEP (data_at sh_r tuint512 (block512_to_vals x_content) x;
          data_at sh_r tuint512 (block512_to_vals y_content) y;
-         data_at sh_w tuint512 (block512_to_vals (LPSX x_content y_content)) z).
+         data_at sh_w tuint512 (block512_to_vals (LPSX x_content y_content)) z;
+         data_at sh_r (tarray (tarray tulong 256) 8) (Ax_to_vals gen_Ax) Ax).
 
 
 Definition inv_data_mem (sh :share) (x : val) (x_content : block512) : mpred :=
@@ -40,9 +56,9 @@ Definition inv_data_mem (sh :share) (x : val) (x_content : block512) : mpred :=
 
 Definition inv_data_mem_res (sh :share) (i : Z) (z : val) (x_content y_content z_content : block512) : mpred :=
   (
-   data_at sh tuint512 (block512_to_vals (int64s_to_block512
-      (sublist 0 i (block512_to_int64s (LPSX x_content y_content)) ++
-                            (sublist i 8 (block512_to_int64s z_content))))) z).
+   data_at sh tuint512 (
+      (sublist 0 i (block512_to_vals (LPSX x_content y_content)) ++
+                            (sublist i 8 (block512_to_vals z_content)))) z).
 
 (*
 Definition A_rev := rev A.
@@ -71,6 +87,7 @@ Fixpoint create_Ax (pi : list byte) (A : list int64) : list (list int64) . *)
 
 
 
+
 Lemma body_streebog_xlps :
   semax_body Vprog [] f_streebog_xlps streebog_xlps_spec.
 Proof.
@@ -83,20 +100,21 @@ Proof.
 
   deadvars!.
   forward_loop
-   (EX i:Z,(*EX j:Z, EX data: list int64,*)
-   PROP( sublist 0 i (block512_to_int64s (LPSX x_content y_content)) =
-            sublist 0 i (block512_to_int64s z_content))
-    (* PROP (0 <= i <= 8 ;
-          0 <= j <=  i ;
-          nth (Z.to_nat j) data default =
-            nth (Z.to_nat j) (block512_to_int64s (LPSX x_content y_content)) Int64.zero) *)
-    LOCAL ( )
-    SEP (inv_data_mem sh_r x x_content; inv_data_mem sh_r y y_content; inv_data_mem_res sh_w i z x_content y_content z_content)
+   (EX i:Z,(*EX j:Z, EX data: list int64,*) 
+    PROP(0 <= i <= 7)
+    LOCAL (temp _i (Vint (Int.repr i)))
+    SEP (inv_data_mem sh_r x x_content; inv_data_mem sh_r y y_content; 
+         inv_data_mem_res sh_w i z x_content y_content z_content;
+         data_at sh_r (tarray (tarray tulong 256) 8) (Ax_to_vals gen_Ax) Ax)
     ).
   - forward.
     entailer!.
-    Exists 0.
-    entailer!.
+    Exists 0. 
+    entailer!. 
+  - hint. Intros i. hint.
+    forward_if.
+    + hint. abbreviate_semax. unfold Ax_to_vals. forward.
+    + 
     unfold inv_data_mem.
     unfold inv_data_mem_res.
     simpl.
